uniqueHeap/ForkIndependence.v
@@ -1,4 +1,4 @@
-Require Import SfLib.       
+Require Import SfLib.        
 Require Import NonSpec.  
 Require Import Spec.  
 Require Import AST. 
@@ -74,12 +74,6 @@ Proof.
     eauto. eauto. }
    {inversion H; subst. 
     {inv H3. eapply IHspec_multistep. apply Union_intror. constructor. eauto. }
-    {inv H3. eapply IHspec_multistep. apply Union_intror. constructor. eauto. }
-    {inv H3. eapply IHspec_multistep. apply Union_intror. constructor. eauto. }
-    {inv H3. eapply IHspec_multistep. apply Union_intror. constructor. eauto. }
-    {inv H3. eapply IHspec_multistep. apply Union_intror. constructor. eauto. }
-    {inv H3. eapply IHspec_multistep. apply Union_intror. constructor. eauto. }
-    {inv H3. eapply IHspec_multistep. apply Union_intror. constructor. eauto. }
     {inv H3. eapply IHspec_multistep with(s4 := aCons (fAct M E M0 d)s1)(s3:=s2) in H2. 
      destruct s1; simpl in *; omega. apply Union_intror. apply Couple_l. }
     {inv H3. eapply IHspec_multistep with(s4:=aCons (rAct x M E d)s1)(s3:=s2) in H2. 
@@ -134,16 +128,6 @@ Proof.
   intros. unfold commitPool. intros. unfoldSetEq H. apply H1 in H0. inv H0. inv H3; inv H4; auto. 
 Qed. 
 
-Theorem forkInd : forall H H' TID s2 M N E d T T' s t,
-                    spec_multistep H
-                                   (tUnion T (tSingleton (TID,unlocked nil,s2,t))) H'
-                                   (tUnion T' (tSingleton(TID,(unlocked(s++[fAct M E N d])), s2, M))) ->
-                    spec_multistep H
-                                   (tUnion T (tSingleton(TID,unlocked nil,fAct M E N d::s2,t))) H'
-                                   (tUnion T' (tSingleton(TID,unlocked s,fAct M E N d::s2,M))).
-Proof.
-Admitted. 
-
 Theorem unspecUnlocked : forall tid s1 s2 M t', 
                    unspecThread (tid,unlocked s1,s2,M) t' ->
                    exists M',  t' = tSingleton (tid, unlocked nil, s2, M'). 
@@ -151,16 +135,95 @@ Proof.
   intros. inv H; eauto. 
 Qed. 
 
-Theorem forkInd' : forall H H' T T' tid M M' M'' N s1 s1' s2 s2' E d,
+
+Ltac eqIn H :=  unfoldTac; 
+  match type of H with
+    | forall x, In ?X (Union ?X ?T (Singleton ?X ?t)) x -> ?z => 
+            assert(In X (Union X T (Singleton X t)) t) by (apply Union_intror; constructor)
+  end. 
+            
+
+Theorem specStepDiffUnused : forall H T H' T' t t',
+                               spec_step H T t H' T t' ->
+                               spec_step H T' t H' T' t'. 
+Proof.
+  intros. inv H0; auto. 
+  {eapply SGet; eauto. }{eapply SPut; eauto. }
+Qed. 
+
+Theorem decomposeNeq : forall M E E' e e', decompose M E e -> decompose M E' e' -> e <> e' ->
+                                           False. 
+Proof.
+  intros. eapply uniqueCtxtDecomp in H; eauto. invertHyp. apply H1. auto.
+Qed. 
+
+Ltac invert := 
+  match goal with
+    |H:?x = ?x |- _ => clear H; invert
+    |H:?x = ?y |- _ => inv H; subst; match goal with
+                                       |H':?x = ?y |- _ => fail
+                                       |_ => idtac
+                                     end 
+  end. 
+
+Theorem forkInd' : forall M M' M'' E N N' h h' T T' s1 s1' s2 d tid,
+      spec_multistep h (tUnion T (tCouple(tid,unlocked[fAct M' E N d], s2, M)
+                                         (1::tid,locked nil, nil, N)))
+                     h' (tUnion T' (tCouple(tid,unlocked(s1++[fAct M' E N d]), s2, M'')
+                                           (1::tid,locked s1', nil, N'))) ->
+      exists h'' T'',
+      spec_multistep h (tUnion T (tCouple(tid,unlocked[fAct M' E N d], s2, M)
+                                         (1::tid,locked nil, nil, N)))
+                     h'' (tUnion T'' (unspecPoolAux(tCouple (tid,unlocked s1,s2,M'')
+                                                            (1::tid,locked s1', nil, N')))) /\
+      spec_multistep h'' (tUnion T''(unspecPoolAux(tCouple (tid,unlocked s1,s2,M'')
+                                                            (1::tid,locked s1', nil, N'))))
+                     h' (tUnion T' (tCouple(tid,unlocked(s1++[fAct M' E N d]), s2, M'')
+                                           (1::tid,locked s1', nil, N'))). 
+Admitted. 
+
+Theorem forkInd : forall H H' T T' tid M M' M'' N s1 s1' s2 E d,
                     spec_multistep H (tUnion T (tSingleton(tid, unlocked [], s2, M'))) H'
                                    (tUnion T' (tCouple(tid, unlocked(s1 ++ [fAct M' E M'' d]), s2, M)
-                                                      (1 :: tid, locked s1', s2', N))) ->
-                    spec_multistep H (tUnion T (unspecPoolAux (tCouple (tid,unlocked s1',fAct M' E M'' d::s2, M)
-                                                                       (1::tid,unlocked s1', s2', N))))
+                                                      (1 :: tid, locked s1', nil, N))) ->
+                    spec_multistep H (tUnion T (unspecPoolAux (tCouple (tid,unlocked s1,fAct M' E M'' d::s2, M)
+                                                                       (1::tid,unlocked s1', nil, N))))
                                    H' (tUnion T' (tCouple(tid,unlocked s1,fAct M' E M'' d::s2, M)
-                                                         (1::tid,unlocked s1', s2', N))).
+                                                         (1::tid,unlocked s1', nil, N))).
 Proof.
-  intros. 
+  intros. dependent induction H0. 
+  {unfoldTac. rewrite couple_swap in x. rewrite coupleUnion in x. 
+   rewrite <- Union_associative in x. apply UnionEqTID in x. invertHyp. inv H. invertListNeq. }
+  {copy H. apply specStepSingleton in H1. invertHyp. copy x. unfoldSetEq x. eqIn H2. 
+   apply H2 in H4. inversion H4; subst. 
+   {copy H5. apply pullOut in H5. rewrite Union_commutative. rewrite H5. rewrite <- Union_associative. 
+    econstructor. eapply specStepDiffUnused. eauto. unfoldTac. rewrite Union_associative.  
+    rewrite (Union_commutative thread _ t'). rewrite Union_commutative.
+    eapply IHspec_multistep; eauto. apply UnionSingletonEq in H1; auto. rewrite H1. 
+    apply EqJMeq. unfoldTac. rewrite Union_associative. rewrite (Union_commutative thread t').
+    rewrite Union_associative. rewrite (Union_commutative thread t'). auto. }
+   {inv H5. apply UnionEqTID in H1. invertHyp. cleanup. inversion H; subst; try solve[
+     unfoldTac; invertHyp; invert; 
+     match goal with
+       |H:decompose ?M ?E ?e,H':decompose ?M ?E' ?e' |- _ => 
+        assert(CONTRA:e <> e') by introsInv
+     end; eapply decomposeNeq in CONTRA; eauto; contradiction].                                                   
+    {inv H5; unfoldTac; invertHyp; inv H1; 
+     match goal with
+       |H:decompose ?M ?E ?e,H':decompose ?M ?E' ?e' |- _ => 
+        assert(CONTRA:e <> e') by introsInv
+     end; eapply decomposeNeq in CONTRA; eauto; contradiction. }
+    {unfoldTac; invertHyp. invert. simpl in *. copy d; copy d0. eapply uniqueCtxtDecomp in H1; eauto.  
+     invertHyp. inv H7. assert(d=d0) by apply proof_irrelevance. subst. apply forkInd' in H0. 
+     invertHyp. 
+
+
+
+apply EqJMeq. fold tUnion. unfoldTac. 
+    rewrite (Union_commutative thread t'). rewrite Union_associative. eapply UnionSingletonEq. 
+
+    
+
 Admitted. 
 (*
 Theorem forkInd'' : forall H N TID s2 M E d T T' s,
